add point_inv to spec

specs/ecc/Spec.EC.Lemmas.fst
@@ -5,7 +5,43 @@ open Spec.EC
 
 #set-options "--z3rlimit 50 --ifuel 0 --fuel 0"
 
+let aff_point_add_inv_lemma k p q = admit()
+
+
+let aff_point_negate_on_curve_lemma k p =
+  let ( +% ) = fadd k in
+  let ( *% ) = fmul k in
+
+  let p_neg = aff_point_negate k p in
+  let px, py = p_neg in
+  let qx, qy = p in
+  assert (px = qx /\ py = (-qy) % prime);
+  assert (is_on_curve k p);
+  assert (qy *% qy == qx *% qx *% qx +% k.coeff_a *% qx +% k.coeff_b);
+  assert (py * py % prime = ((-qy) % prime * ((-qy) % prime)) % prime);
+  Math.Lemmas.lemma_mod_mul_distr_l (-qy) ((-qy) % prime) prime;
+  Math.Lemmas.lemma_mod_mul_distr_r (-qy) (-qy) prime;
+  assert (py * py % prime = ((-qy) * (-qy)) % prime);
+  Math.Lemmas.neg_mul_left qy (-qy);
+  assert (py * py % prime = (- (qy * (-qy))) % prime);
+  Math.Lemmas.neg_mul_right qy qy;
+  assert (py * py % prime = (qy * qy) % prime);
+  assert (is_on_curve k p_neg)
+
+
+let aff_point_negate_inv_lemma k p =
+  let p_neg = aff_point_negate k p in
+  let px, py = p_neg in
+  let qx, qy = p in
+  assert (px = qx /\ py = (-qy) % prime);
+
+  if is_aff_point_at_inf k p then
+    assert (is_aff_point_at_inf k p_neg)
+  else aff_point_negate_on_curve_lemma k p
+
+
 let aff_point_at_inf_lemma (k:curve) (p:aff_point k) = ()
+
 
 let aff_point_add_assoc_lemma (k:curve) (p q s:aff_point k) = admit()
 
