specs/ecc/Spec.EC.Projective.Lemmas.fst
@@ -3,68 +3,11 @@ module Spec.EC.Projective.Lemmas
 open FStar.Mul
 
 module M = Lib.NatMod
+module SL = Spec.EC.Lemmas
 
 open Spec.EC.Projective
 
 #set-options "--z3rlimit 50 --fuel 0 --ifuel 0"
-
-let lemma_aff_is_point_at_inf k p =
-  k.prime_lemma ();
-  let (px, py, pz) = p in
-  M.lemma_div_mod_prime_is_zero #prime px pz;
-  M.lemma_div_mod_prime_is_zero #prime py pz
-
-
-let lemma_proj_aff_id k p =
-  let (px, py) = p in
-  let (pX, pY, pZ) = to_proj_point k p in
-  assert (pX = px /\ pY = pY /\ pZ = 1);
-  let (rx, ry) = to_aff_point k (pX, pY, pZ) in
-  assert (rx = fmul k pX (finv k pZ) /\ ry = fmul k pY (finv k pZ));
-  M.lemma_div_mod_prime_one #prime pX;
-  M.lemma_div_mod_prime_one #prime pY;
-  assert (rx = pX /\ ry = pY)
-
-
-let to_aff_point_at_infinity_lemma k =
-  let px, py = to_aff_point k (point_at_inf k) in
-  assert (px == fmul k 0 (finv k 0) /\ py == fmul k 1 (finv k 0));
-  assert (px == fmul k 0 (M.pow_mod #prime 0 (prime - 2)));
-  M.lemma_pow_mod #prime 0 (prime - 2);
-  assert (px == fmul k 0 (M.pow 0 (prime - 2) % prime));
-  M.lemma_pow_zero (prime - 2);
-  assert (px == 0 /\ py == 0)
-
-
-let to_aff_point_negate_lemma k p =
-  let px, py, pz = p in
-  let qx, qy = to_aff_point k (point_negate k p) in
-  assert (qx == fmul k px (finv k pz) /\ qy == fmul k ((- py) % prime) (finv k pz));
-  let ax, ay = aff_point_negate k (to_aff_point k p) in
-  assert (ax == fmul k px (finv k pz) /\ ay == (- (fmul k py (finv k pz))) % prime);
-  let pz_inv = M.pow_mod #prime pz (prime - 2) in
-
-  calc (==) { // (-py) % prime /% pz;
-    ((- py) % k.prime * pz_inv) % k.prime;
-    (==) { Math.Lemmas.lemma_mod_mul_distr_l (- py) pz_inv k.prime }
-    ((- py) * pz_inv) % k.prime;
-    (==) { Math.Lemmas.neg_mul_left py pz_inv }
-    (- (py * pz_inv)) % k.prime;
-    (==) { Math.Lemmas.lemma_mod_sub_distr 0 (py * pz_inv) k.prime }
-    (- (py * pz_inv) % k.prime) % k.prime; // (- py /% pz) % prime;
-  }
-
-
-let to_aff_point_add_lemma_a3 k p q = admit()
-
-let to_aff_point_double_lemma_a3 k p = admit()
-
-
-let to_aff_point_add_lemma_a0 k p q = admit()
-
-let to_aff_point_double_lemma_a0 k p = admit()
-
-//-------------------------------
 
 val lemma_div_mod_eq_mul_mod (k:curve) (a b c:felem k) : Lemma
   (requires b <> 0)
@@ -139,3 +82,68 @@ let ecdsa_verify_avoid_finv2 k p r =
 let ecdsa_verify_avoid_finv k p r =
   ecdsa_verify_avoid_finv1 k p r;
   ecdsa_verify_avoid_finv2 k p r
+
+//-----------------------------------------
+
+let lemma_aff_is_point_at_inf k p =
+  k.prime_lemma ();
+  let (px, py, pz) = p in
+  M.lemma_div_mod_prime_is_zero #prime px pz;
+  M.lemma_div_mod_prime_is_zero #prime py pz
+
+
+let lemma_proj_aff_id k p =
+  let (px, py) = p in
+  let (pX, pY, pZ) = to_proj_point k p in
+  assert (pX = px /\ pY = pY /\ pZ = 1);
+  let (rx, ry) = to_aff_point k (pX, pY, pZ) in
+  assert (rx = fmul k pX (finv k pZ) /\ ry = fmul k pY (finv k pZ));
+  M.lemma_div_mod_prime_one #prime pX;
+  M.lemma_div_mod_prime_one #prime pY;
+  assert (rx = pX /\ ry = pY)
+
+
+let to_aff_point_at_infinity_lemma k =
+  let px, py = to_aff_point k (point_at_inf k) in
+  assert (point_at_inf k = (0, 1, 0));
+  let zinv = finv k 0 in
+  assert (px == fmul k 0 zinv /\ py == fmul k 1 zinv);
+  assert (zinv == M.pow_mod #prime 0 (prime - 2));
+  M.lemma_pow_mod #prime 0 (prime - 2);
+  assert (zinv == M.pow 0 (prime - 2) % prime);
+  assert (prime > 2);
+  M.lemma_pow_zero (prime - 2);
+  assert (zinv == 0);
+  assert (px == 0 /\ py == 0)
+
+
+let to_aff_point_negate_lemma k p =
+  let px, py, pz = p in
+  let qx, qy = to_aff_point k (point_negate k p) in
+  assert (qx == fmul k px (finv k pz) /\ qy == fmul k ((- py) % prime) (finv k pz));
+  let ax, ay = aff_point_negate k (to_aff_point k p) in
+  assert (ax == fmul k px (finv k pz) /\ ay == (- (fmul k py (finv k pz))) % prime);
+  let pz_inv = M.pow_mod #prime pz (prime - 2) in
+
+  calc (==) { // (-py) % prime /% pz;
+    ((- py) % k.prime * pz_inv) % k.prime;
+    (==) { Math.Lemmas.lemma_mod_mul_distr_l (- py) pz_inv k.prime }
+    ((- py) * pz_inv) % k.prime;
+    (==) { Math.Lemmas.neg_mul_left py pz_inv }
+    (- (py * pz_inv)) % k.prime;
+    (==) { Math.Lemmas.lemma_mod_sub_distr 0 (py * pz_inv) k.prime }
+    (- (py * pz_inv) % k.prime) % k.prime; // (- py /% pz) % prime;
+  };
+  assert (to_aff_point k (point_negate k p) == aff_point_negate k (to_aff_point k p));
+  Spec.EC.Lemmas.aff_point_negate_inv_lemma k (to_aff_point k p);
+  assert (point_inv k (point_negate k p))
+
+
+let to_aff_point_add_lemma_a3 k p q = admit()
+
+let to_aff_point_double_lemma_a3 k p = admit()
+
+
+let to_aff_point_add_lemma_a0 k p q = admit()
+
+let to_aff_point_double_lemma_a0 k p = admit()
