specs/ecc/Spec.ECC.Projective.fst
@@ -12,42 +12,52 @@ include Spec.EC.Projective
 
 #set-options "--z3rlimit 50 --fuel 0 --ifuel 0"
 
+
 ///  Elliptic curve scalar multiplication
 
-let mk_to_ec_comm_monoid (k:curve) : SE.to_comm_monoid (proj_point k) = {
-  SE.a_spec = aff_point k;
+let mk_to_ec_comm_monoid (k:curve) : SE.to_comm_monoid (proj_point_c k) = {
+  SE.a_spec = aff_point_c k;
   SE.comm_monoid = EC.mk_ec_comm_monoid k;
-  SE.refl = to_aff_point k;
+  SE.refl = (fun (x:proj_point_c k) -> to_aff_point k x);
 }
 
-val point_at_inf_c: k:curve -> SE.one_st (proj_point k) (mk_to_ec_comm_monoid k)
+val point_at_inf_c: k:curve -> SE.one_st (proj_point_c k) (mk_to_ec_comm_monoid k)
 let point_at_inf_c k _ =
   EPL.to_aff_point_at_infinity_lemma k;
   point_at_inf k
 
 
-let is_point_at_inf_c (k:curve) (p:proj_point k)
+let is_point_at_inf_c (k:curve) (p:proj_point_c k)
   : res:bool{res ==> EC.is_aff_point_at_inf k (to_aff_point k p)}
  =
   EPL.lemma_aff_is_point_at_inf k p;
   is_point_at_inf k p
 
 
+let to_proj_point_c (k:curve) (p:aff_point_c k) : proj_point_c k =
+  let px, py = p in
+  k.prime_lemma ();
+  Lib.NatMod.lemma_div_mod_prime_one #k.prime px;
+  Lib.NatMod.lemma_div_mod_prime_one #k.prime py;
+  to_proj_point k p
+
+
 ///  for elliptic curve with coeff_a = (-3) % prime
 
 val point_add_c_a3: k:curve{k.coeff_a = (-3) % k.prime}
-  -> SE.mul_st (proj_point k) (mk_to_ec_comm_monoid k)
+  -> SE.mul_st (proj_point_c k) (mk_to_ec_comm_monoid k)
 let point_add_c_a3 k p q =
   EPL.to_aff_point_add_lemma_a3 k p q;
   point_add_a3 k p q
 
 val point_double_c_a3: k:curve{k.coeff_a = (-3) % k.prime}
-  -> SE.sqr_st (proj_point k) (mk_to_ec_comm_monoid k)
+  -> SE.sqr_st (proj_point_c k) (mk_to_ec_comm_monoid k)
 let point_double_c_a3 k p =
   EPL.to_aff_point_double_lemma_a3 k p;
   point_double_a3 k p
 
-let mk_ec_concrete_ops_a3 (k:curve{k.coeff_a = (-3) % k.prime}) : SE.concrete_ops (proj_point k) =
+let mk_ec_concrete_ops_a3 (k:curve{k.coeff_a = (-3) % k.prime})
+  : SE.concrete_ops (proj_point_c k) =
 {
   SE.to = mk_to_ec_comm_monoid k;
   SE.one = point_at_inf_c k;
@@ -58,17 +68,19 @@ let mk_ec_concrete_ops_a3 (k:curve{k.coeff_a = (-3) % k.prime}) : SE.concrete_op
 
 ///  for elliptic curve with coeff_a = 0
 
-val point_add_c_a0: k:curve{k.coeff_a = 0} -> SE.mul_st (proj_point k) (mk_to_ec_comm_monoid k)
+val point_add_c_a0: k:curve{k.coeff_a = 0}
+  -> SE.mul_st (proj_point_c k) (mk_to_ec_comm_monoid k)
 let point_add_c_a0 k p q =
   EPL.to_aff_point_add_lemma_a0 k p q;
   point_add_a0 k p q
 
-val point_double_c_a0: k:curve{k.coeff_a = 0} -> SE.sqr_st (proj_point k) (mk_to_ec_comm_monoid k)
+val point_double_c_a0: k:curve{k.coeff_a = 0}
+  -> SE.sqr_st (proj_point_c k) (mk_to_ec_comm_monoid k)
 let point_double_c_a0 k p =
   EPL.to_aff_point_double_lemma_a0 k p;
   point_double_a0 k p
 
-let mk_ec_concrete_ops_a0 (k:curve{k.coeff_a = 0}) : SE.concrete_ops (proj_point k) =
+let mk_ec_concrete_ops_a0 (k:curve{k.coeff_a = 0}) : SE.concrete_ops (proj_point_c k) =
 {
   SE.to = mk_to_ec_comm_monoid k;
   SE.one = point_at_inf_c k;
@@ -85,8 +97,8 @@ let is_supported (k:curve) =
 
 
 // [a]P
-let point_mul (k:curve{is_supported k}) (a:qelem k) (p:proj_point k)
-  : res:proj_point k{to_aff_point k res == EC.aff_point_mul k a (to_aff_point k p) }
+let point_mul (k:curve{is_supported k}) (a:qelem k) (p:proj_point_c k)
+  : res:proj_point_c k{to_aff_point k res == EC.aff_point_mul k a (to_aff_point k p) }
  =
   let aBits = 8 * k.order_len_bytes in // TODO: add order_bits to `curve`?
   let w = 4 in // TODO: use montgomery ladder for the spec?
@@ -101,8 +113,8 @@ let point_mul (k:curve{is_supported k}) (a:qelem k) (p:proj_point k)
 
 
 // [a1]G + [a2]P
-let point_mul_double_g (k:curve{is_supported k}) (a1 a2:qelem k) (p:proj_point k)
-  : res:proj_point k{to_aff_point k res ==
+let point_mul_double_g (k:curve{is_supported k}) (a1 a2:qelem k) (p:proj_point_c k)
+  : res:proj_point_c k{to_aff_point k res ==
       EC.aff_point_add k
         (EC.aff_point_mul k a1 k.base_point) (EC.aff_point_mul k a2 (to_aff_point k p)) }
  =
@@ -124,9 +136,9 @@ let point_mul_double_g (k:curve{is_supported k}) (a1 a2:qelem k) (p:proj_point k
 
 let ec_concrete_ops_proj (k:curve{is_supported k}) : EC.ec_concrete_ops = {
   EC.ec = k;
-  EC.t = proj_point k;
-  EC.to_point_t = to_proj_point k;
-  EC.to_aff_point = to_aff_point k;
+  EC.t = proj_point_c k;
+  EC.to_point_t = to_proj_point_c k;
+  EC.to_aff_point = (fun (x:proj_point_c k) -> to_aff_point k x);
   EC.lemma_to_from_aff_point = EPL.lemma_proj_aff_id k;
   EC.is_point_at_inf = is_point_at_inf_c k;
   EC.point_mul = point_mul k;
