specs/ecc/Spec.EC.Projective.Lemmas.fsti
@@ -5,12 +5,15 @@ open Spec.EC.Projective
 
 #set-options "--z3rlimit 50 --fuel 0 --ifuel 0"
 
-(** The point addition and doubling formulas are taken from
-    https://eprint.iacr.org/2015/1060.pdf. The correctness of
-    the formulas is shown in Appendix A of the paper. Their
-    verification in F* is left for the future. *)
+// works when q < prime /\ prime < 2 * q
+val ecdsa_verify_avoid_finv:
+    k:curve{k.order < k.prime /\ k.prime < 2 * k.order}
+  -> p:proj_point k{not (is_point_at_inf k p)}
+  -> r:nat{0 < r /\ r < k.order} ->
+  Lemma (let _X, _Y, _Z = p in
+    (fmul k _X (finv k _Z) % k.order = r) <==>
+    ((fmul k r _Z = _X) || (r + k.order < k.prime && fmul k (r + k.order) _Z = _X)))
 
-// TODO: add `point_inv p = is_on_curve p || is_point_at_inf p`
 
 val lemma_aff_is_point_at_inf: k:curve -> p:proj_point k ->
   Lemma (let px, py, pz = p in
@@ -25,35 +28,31 @@ val to_aff_point_at_infinity_lemma: k:curve ->
   Lemma (to_aff_point k (point_at_inf k) == aff_point_at_inf k)
 
 
-val to_aff_point_negate_lemma (k:curve) (p:proj_point k) :
-  Lemma (to_aff_point k (point_negate k p) == aff_point_negate k (to_aff_point k p))
+val to_aff_point_negate_lemma (k:curve) (p:proj_point_c k) :
+  Lemma (point_inv k (point_negate k p) /\
+    to_aff_point k (point_negate k p) == aff_point_negate k (to_aff_point k p))
 
 
-val to_aff_point_add_lemma_a3 (k:curve{k.coeff_a = (-3) % k.prime}) (p q:proj_point k) :
-  Lemma (to_aff_point k (point_add_a3 k p q) ==
-    aff_point_add k (to_aff_point k p) (to_aff_point k q))
+(** The point addition and doubling formulas are taken from
+    https://eprint.iacr.org/2015/1060.pdf. The correctness of
+    the formulas is shown in Appendix A of the paper. Their
+    verification in F* is left for the future. *)
+
+val to_aff_point_add_lemma_a3 (k:curve{k.coeff_a = (-3) % k.prime}) (p q:proj_point_c k) :
+  Lemma (point_inv k (point_add_a3 k p q) /\
+    to_aff_point k (point_add_a3 k p q) == aff_point_add k (to_aff_point k p) (to_aff_point k q))
 
 
-val to_aff_point_double_lemma_a3 (k:curve{k.coeff_a = (-3) % k.prime}) (p:proj_point k) :
-  Lemma (to_aff_point k (point_double_a3 k p) ==
-    aff_point_add k (to_aff_point k p) (to_aff_point k p))
+val to_aff_point_double_lemma_a3 (k:curve{k.coeff_a = (-3) % k.prime}) (p:proj_point_c k) :
+  Lemma (point_inv k (point_double_a3 k p) /\
+    to_aff_point k (point_double_a3 k p) == aff_point_add k (to_aff_point k p) (to_aff_point k p))
 
 
-val to_aff_point_add_lemma_a0 (k:curve{k.coeff_a = 0}) (p q:proj_point k) :
-  Lemma (to_aff_point k (point_add_a0 k p q) ==
-    aff_point_add k (to_aff_point k p) (to_aff_point k q))
+val to_aff_point_add_lemma_a0 (k:curve{k.coeff_a = 0}) (p q:proj_point_c k) :
+  Lemma (point_inv k (point_add_a0 k p q) /\
+    to_aff_point k (point_add_a0 k p q) == aff_point_add k (to_aff_point k p) (to_aff_point k q))
 
 
-val to_aff_point_double_lemma_a0 (k:curve{k.coeff_a = 0}) (p:proj_point k) :
-  Lemma (to_aff_point k (point_double_a0 k p) ==
-    aff_point_add k (to_aff_point k p) (to_aff_point k p))
-
-
-// works when q < prime /\ prime < 2 * q
-val ecdsa_verify_avoid_finv:
-    k:curve{k.order < k.prime /\ k.prime < 2 * k.order}
-  -> p:proj_point k{not (is_point_at_inf k p)}
-  -> r:nat{0 < r /\ r < k.order} ->
-  Lemma (let _X, _Y, _Z = p in
-    (fmul k _X (finv k _Z) % k.order = r) <==>
-    ((fmul k r _Z = _X) || (r + k.order < k.prime && fmul k (r + k.order) _Z = _X)))
+val to_aff_point_double_lemma_a0 (k:curve{k.coeff_a = 0}) (p:proj_point_c k) :
+  Lemma (point_inv k (point_double_a0 k p) /\
+    to_aff_point k (point_double_a0 k p) == aff_point_add k (to_aff_point k p) (to_aff_point k p))
